rm old select/selectl/selectf/selectfs

backend/Selectionaux.ml
@@ -75,9 +75,9 @@ let fast_cmove ty =
   | "powerpc", _ -> false
   | "riscV", _ -> false
   | "x86", _ -> 
-      (match ty with Tint -> true | Tlong -> Archi.ptr64 | _ -> false)
-  | _, _ ->
-      assert false
+     (match ty with Tint -> true | Tlong -> Archi.ptr64 | _ -> false)
+  | "mppa_k1c", _ -> false (* TODO DM *)
+  | a, m -> failwith (Printf.sprintf "fast_cmove: unknown arch %s %s" a m)
 
 (* The if-conversion heuristic depend on the
    -fif-conversion and -ffavor-branchless flags.
