mppa_k1c/Asmblockgen.v
@@ -784,31 +784,10 @@ Definition transl_op
   | Olonguofsingle , _ => Error (msg "Asmblockgen.transl_op: Olonguofsingle")
 
 
-
   | Ocmp cmp, _ =>
       do rd <- ireg_of res;
       transl_cond_op cmp rd args k
 
-  | Oselect cond, a0 :: a1 :: aS :: nil
-  | Oselectl cond, a0 :: a1 :: aS :: nil
-  | Oselectf cond, a0 :: a1 :: aS :: nil
-  | Oselectfs cond, a0 :: a1 :: aS :: nil  =>
-    assertion (mreg_eq a0 res);
-      do r0 <- ireg_of a0;
-      do r1 <- ireg_of a1;
-      do rS <- ireg_of aS;
-      (match cond with
-       | Ccomp0 cmp =>
-         OK (Pcmove (btest_for_cmpswz cmp) r0 rS r1 ::i k)
-       | Ccompu0 cmp =>
-         do bt <- btest_for_cmpuwz cmp;
-           OK (Pcmoveu bt r0 rS r1 ::i k)
-       | Ccompl0 cmp =>
-         OK (Pcmove (btest_for_cmpsdz cmp) r0 rS r1 ::i k)
-       | Ccomplu0 cmp =>
-         do bt <- btest_for_cmpudz cmp;
-           OK (Pcmoveu bt r0 rS r1 ::i k)
-       end)
 
   | Oextfz stop start, a1 :: nil =>
     assertion (ExtValues.is_bitfield stop start);
